platform/cito/Inv.v
@@ -13,18 +13,17 @@ Section layout.
 
   Variable layout : Layout.
 
-  Definition has_extra_stack sp offset :=
-    (Ex stack,
-     (sp ^+ $4) =*> stack *
-     (sp ^+ $8 ^+ $(4 * offset)) =?> (wordToNat stack))%Sep.
+  Definition has_extra_stack sp offset e_stack :=
+    ((sp ^+ $4) =*> $(e_stack) *
+     (sp ^+ $8 ^+ $(4 * offset)) =?> e_stack)%Sep.
 
-  Definition is_state sp rp vars (v : State) temps : HProp :=
+  Definition is_state sp rp e_stack vars (v : State) temps : HProp :=
     (
      locals vars (fst v) 0 (sp ^+ $8) *
      array temps (sp ^+ $8 ^+ $(4 * length vars)) *
      is_heap layout (snd v) *
      sp =*> rp *
-     has_extra_stack sp (length vars + length temps)
+     has_extra_stack sp (length vars + length temps) e_stack
     )%Sep.
 
   Require Import Malloc.
@@ -59,13 +58,13 @@ Section layout.
     ((Al i, Al spec, 
       [| fs i = Some (Internal spec) |] 
         ---> (i, stn) @@@ (
-          st ~> ExX, Ex v, Ex rp,
-          ![^[is_state st#Sp rp (ArgVars spec) v nil * mallocHeap 0] * #0] st /\
+          st ~> ExX, Ex v, Ex rp, Ex e_stack,
+          ![^[is_state st#Sp rp e_stack (ArgVars spec) v nil * mallocHeap 0] * #0] st /\
           [| Safe fs (Body spec) v |] /\
           (st#Rp, stn) 
             @@@ (
               st' ~> Ex v', Ex rp',
-              ![^[ is_state st'#Sp rp' (ArgVars spec) v' nil * mallocHeap 0] * #1] st' /\
+              ![^[ is_state st'#Sp rp' e_stack (ArgVars spec) v' nil * mallocHeap 0] * #1] st' /\
               [| exists vs', 
                  RunsTo fs (Body spec) v (vs', snd v') /\ 
                  st'#Rv = sel vs' (RetVar spec) /\
@@ -73,8 +72,8 @@ Section layout.
      (Al i, Al spec, 
       [| fs i = Some (Foreign spec) |] 
         ---> (i, stn) @@@ (
-          st ~> ExX, Ex heap, Ex pairs, Ex rp,
-          ![^[is_state st#Sp rp nil (empty_vs, heap) (map fst pairs) * mallocHeap 0] * #0] st /\
+          st ~> ExX, Ex heap, Ex pairs, Ex rp, Ex e_stack,
+          ![^[is_state st#Sp rp e_stack nil (empty_vs, heap) (map fst pairs) * mallocHeap 0] * #0] st /\
           [| List.Forall (heap_match heap) pairs /\
              PreCond spec (map snd pairs) |] /\
           (st#Rp, stn) 
@@ -83,7 +82,7 @@ Section layout.
               let t := decide_ret addr ret in
               let ret_w := fst t in
               let ret_a := snd t in
-              ![^[is_state st#Sp rp' nil (empty_vs, heap') args' * layout_option addr ret_a * mallocHeap 0] * #1] st' /\
+              ![^[is_state st#Sp rp' e_stack nil (empty_vs, heap') args' * layout_option addr ret_a * mallocHeap 0] * #1] st' /\
               [| length outs = length pairs /\
                  let triples := make_triples pairs outs in
                  PostCond spec (map (fun x => (Semantics.In x, Out x)) triples) ret /\
@@ -103,14 +102,14 @@ Section layout.
     Definition inv_template precond postcond get_sp : assert := 
       st ~> Ex fs, 
       funcs_ok (fst st) fs /\
-      ExX, Ex v, Ex temps, Ex rp,
-      ![^[is_state (get_sp st) rp vars v temps * mallocHeap 0] * #0] st /\
+      ExX, Ex v, Ex temps, Ex rp, Ex e_stack,
+      ![^[is_state (get_sp st) rp e_stack vars v temps * mallocHeap 0] * #0] st /\
       [| precond fs v st /\
          length temps = temp_size |] /\
       (rp, fst st) 
         @@@ (
           st' ~> Ex v', Ex temps',
-          ![^[is_state st'#Sp rp vars v' temps' * mallocHeap 0] * #1] st' /\
+          ![^[is_state st'#Sp rp e_stack vars v' temps' * mallocHeap 0] * #1] st' /\
           [| postcond fs v st v' /\
              length temps' = temp_size /\
              st'#Sp = get_sp st |]).
